#+title: Proposition 2.3.4

*Propostion 2.3.4* (Distributive law). /For any natural numbers/ $a,b,c$, /we have/ $a(b+c)=ab+ac$ /and/ $(b+c)a=ba+ca$.

$Proof~by~Tao$. Since multiplication is commutative we only need to show the first identity $a(b+c)=ab+ac$. We keep $a$ and $b$ fixed, and use induction on $c$. Let's prove the base case $c=0$, i.e., $a(b+0)=ab+a0$. The left-hand side is $ab$, while the right-hand side is $ab+0=ab$, so we are done with the base case. Now let us suppose inductively that $a(b+c)=ab+ac$, and let us prove that $a(b+(c\pp))=ab+a(c\pp)$. The left hand ise is $a((b+c)\pp) = a(b+c)+a$, while the right-hand side is $ab+ac+a=a(b+c)+a$ by the induction hypothesis, and so we can close the induction. $\square$
