#+title: Proposition 4.1.6

#+LATEX_HEADER: \usepackage{amsmath}
#+LATEX_HEADER: \usepackage{amssymb}
#+LATEX_HEADER: \usepackage{a4wide}
#+LATEX_HEADER: \renewcommand{\labelitemi}{}
#+LATEX_HEADER: \renewcommand{\labelitemii}{}
#+LATEX_HEADER: \renewcommand{\labelitemiii}{}
#+LATEX_HEADER: \renewcommand{\labelitemiv}{}
#+LaTeX_HEADER: \newcommand{\pp}{\hspace{-0.5pt}{+}\hspace{-4pt}{+}}
#+LaTeX_HEADER: \usepackage[utf8]{inputenc} \usepackage{titlesec}
#+LaTeX_HEADER: \titleformat{\chapter}[block]{\bfseries\Huge}{}{0em}{}
#+LaTeX_HEADER: \titleformat{\section}[hang]{\bfseries\Large}{}{1em}{\thesection\enspace}
#+OPTIONS: num:nil
#+HTML_HEAD: <style type="text/css">
#+HTML_HEAD:  ol#al { list-style-type: upper-alpha; }
#+HTML_HEAD: </style>

*Proposition 4.1.6 (Laws of algebra for integers)*. /Let $x, y, z$ be integers. Then we
have/

  $$
  x + y = y + x
  $$
  
  $$
  (x + y) + z = x + (y + z)
  $$
  
  $$
  x + 0 = 0 + x = x
  $$
  
  $$
  x + (−x) = (−x) + x = 0
  $$
  
  $$
  xy = yx
  $$
  
  $$
  (xy)z = x(yz)
  $$
  
  $$
  x1 = 1x = x
  $$
  
  $$
  x(y + z) = xy + xz
  $$
  
  $$
  (y + z)x = yx + zx
  $$
