#+title: Exercise 3.3.1

 *Exercise 3.3.1.* Show that the definition of equality in [[../definition-3.3.7.org][Definition 3.3.7]] is reflexive, symmetric, and transitive. Also verity the substitution property: if $f,\tilde{f}:X\to Y$ and $g,\tilde{g}:Y\to Z$ are functions such that $f=\tilde{f}$ and $g=\tilde{g}$, then $g\circ f=\tilde{g}\circ\tilde{f}$.
\\

- $+$ Notation: $\text{Domain}(f:X\to Y)= X$
- $+$ Notation: $\text{Range}(f:X\to Y)=Y$

[[../../Appendix/AxiomOfEquality.org][Reflexive]]
- $\bullet$ Show that $\forall f,~f=f$
- $\Vdash$ $f=f$
- $\equiv$ { Claim 1, Claim2, Claim 3, and [[../definition-3.3.7.org][Definition 3.3.7]] }
  - $\text{True}$
- $\square$
  - $\bullet$ Claim 1: $\text{Domain}(f)=\text{Domain}(f)$
  - -- $f:X\to Y$
  - $\Vdash$ $X=X$
  - $\equiv$ { $X$ is an object by [[../axiom-3.1.org][Axiom 3.1]],\\
          $~~~$ [[../../Appendix/AxiomOfEquality.org][reflexive axiom]] for any object }
    - $\text{True}$
  - $\square$
  - $\bullet$ Claim 2: $\text{Range}(f)=\text{Range}(f)$
  - -- $f:X\to Y$
  - $\Vdash$ $Y=Y$
  - $\equiv$ { $Y$ is an object by [[../axiom-3.1.org][Axiom 3.1]],\\
          $~~$ [[../../Appendix/AxiomOfEquality.org][reflexive axiom]] for any object }
    - $\text{True}$
  - $\square$
  - $\bullet$ Claim 3: $\forall x \in X,~f(x)=f(x)$
  - $\Vdash$ $f(x)=f(x)$
  - $\equiv$  { $f(x)$ is an object by [[../definition-3.3.1.org][definition of function]],\\
               $~~~$ [[../../Appendix/AxiomOfEquality.org][reflexive axiom]] for any object  }
    - $\text{True}$
  - $\square$
  \\

[[../../Appendix/AxiomOfEquality.org][Symmetric]]
- $\bullet$ Show that $f=g\implies g=f$
- $\Vdash$ $f=g$
- $\Rightarrow$ { Claim1, Claim2, Claim3 and  [[../definition-3.3.7.org][Definition 3.3.7]] }
  - $g=f$
- $\square$
  - $\bullet$ Claim 1: $\text{Domain}(f)=\text{Domain}(g)\implies\text{Domain}(g)=\text{Domain}(f)$
  - -- $f:X\to Y$
  - -- $g:X'\to Y'$
  - $\Vdash$ $X=X'$
  - $\Rightarrow$ { $X$ and $X'$ are objects by [[../axiom-3.1.org][Axiom 3.1]],\\
          $~~~$ [[../../Appendix/AxiomOfEquality.org][symmetry axiom]] for any two objects of the same type }
    - $X'=X$
  - $\square$
  - $\bullet$ Claim 2: $\text{Range}(f)=\text{Range}(g)\implies\text{Range}(g)=\text{Range}(f)$
  - -- $f:X\to Y$
  - -- $g:X'\to Y'$
  - $\Vdash$ $Y=Y'$
  - $\Rightarrow$ { $X$ and $X'$ are objects by [[../axiom-3.1.org][Axiom 3.1]],\\
          $~~~$ [[../../Appendix/AxiomOfEquality.org][symmetry axiom]] for any two objects of the same type }
    - $Y'=Y$
  - $\square$
  - $\bullet$ Claim 3: $\forall x \in X,~f(x)=g(x)\implies \forall x \in X,~g(x)=f(x)$
  - $\Vdash$ $f(x)=g(x)$
  - $\Rightarrow$ { $f(x)$ and $g(x)$ are objects by [[../definition-3.3.1.org][definition of function]],\\
               $~~~$ the [[../../Appendix/AxiomOfEquality.org][symmetry axiom]] for any two objects of the same type  }
    - $g(x)=f(x)$
  - $\square$
\\

[[../../Appendix/AxiomOfEquality.org][Transitive]]
- $\bullet$ Show that $(f=g)\land(g=h)\implies f=h$
- $\Vdash$ $(f=g)\land(g=h)$
- $\Rightarrow$ { Claim1, Claim2, Claim3 and  [[../definition-3.3.7.org][Definition 3.3.7]] }
  - $f=h$
- $\square$
  - $\bullet$ Claim 1: $(\text{Domain}(f)=\text{Domain}(g))\land(\text{Domain}(g)=\text{Domain}(h))\implies\text{Domain}(f)=\text{Domain}(h)$
  - -- $f:X\to Y$
  - -- $g:X'\to Y'$
  - -- $h:X''\to Y''$
  - $\Vdash$ $X$
  - $=$ { $\text{Domain}(f)=\text{Domain}(g)$ }
    - $X'$
  - $=$ { $\text{Domain}(g)=\text{Domain}(h)$ }
    - $X''$
  - $\Rightarrow$ { $X$, $X'$ and $X''$ are objects by [[../axiom-3.1.org][Axiom 3.1]],\\
          $~~~$ [[../../Appendix/AxiomOfEquality.org][transitive axiom]] for any three objects of the same type }
    - $X=X''$
  - $\square$
  - $\bullet$ Claim 2: $(\text{Range}(f)=\text{Range}(g))\land(\text{Range}(g)=\text{Range}(h))\implies\text{Range}(f)=\text{Range}(h)$
  - -- $f:X\to Y$
  - -- $g:X'\to Y'$
  - -- $h:X''\to Y''$
  - $\Vdash$ $Y$
  - $=$ { $\text{Range}(f)=\text{Range}(g)$ }
    - $Y'$
  - $=$ { $\text{Range}(g)=\text{Range}(h)$ }
    - $Y''$
  - $\Rightarrow$ { $Y$, $Y'$ and $Y''$ are objects by [[../axiom-3.1.org][Axiom 3.1]],\\
          $~~~$ [[../../Appendix/AxiomOfEquality.org][transitive axiom]] for any three objects of the same type }
    - $Y=Y''$
  - $\square$
  - $\bullet$ Claim 3: $(\forall x \in X,~(f(x)=g(x)))\land (\forall x \in X,~(g(x)=h(x))) \implies (\forall x \in X,~f(x)=h(x))$
  - $\Vdash$ $f(x)$
  - $=$ { $f(x)=g(x)$ }
    - $g(x)$
  - $=$ { $g(x)=h(x)$ }
    - $h(x)$
  - $\Rightarrow$ { $f(x)$, $g(x)$ and $h(x)$ are objects by [[../definition-3.3.1.org][definition of function]],\\
           $~~~$ [[../../Appendix/AxiomOfEquality.org][transitive axiom]] for any three objects of the same type }
    - $f(x)=h(x)$
  - $\square$


  [[../../Appendix/AxiomOfEquality.org][Substitution]]
  - $\bullet$ Show that $g\circ f=\tilde{g}\circ\tilde{f}$.
  - -- $f,\tilde{f}:X\to Y$
  - -- $g,\tilde{g}:Y\to Z$
  - $\Vdash$ $g\circ f$
  - $=$ { Claim 1, Claim 2, Claim 3, [[../definition-3.3.7.org][Definition 3.3.7]] and [[../definition-3.3.10.org][Definition 3.3.10]] }
    - $\tilde{g}\circ\tilde{f}$
  - $\square$
    - $\bullet$ Claim 1: $\text{Domain}(g\circ f)=\text{Domain}(\tilde{g}\circ\tilde{f})$
    - $\Vdash$ $\text{Domain}(g\circ f)=\text{Domain}(\tilde{g}\circ\tilde{f})$
    - $\equiv$ { [[../definition-3.3.10.org][Definition 3.3.10 ]] }
      - $X=X$
    - $\equiv$ { $X$ is an objects by [[../axiom-3.1.org][Axiom 3.1]],\\
                 $~~~$ [[../../Appendix/AxiomOfEquality.org][reflexive axiom]] for any object }
      - $\text{True}$
    - $\square$
    - $\bullet$ Claim 2: $\text{Range}(g\circ f)=\text{Range}(\tilde{g}\circ\tilde{f})$
    - $\Vdash$ $\text{Range}(g\circ f)=\text{Range}(\tilde{g}\circ\tilde{f})$
    - $\equiv$ { [[../definition-3.3.10.org][Definition 3.3.10 ]] }
      - $Y=Y$
    - $\equiv$ { $Y$ is an objects by [[../axiom-3.1.org][Axiom 3.1]],\\
                 $~~~$ [[../../Appendix/AxiomOfEquality.org][reflexive axiom]] for any object }
      - $\text{True}$
    - $\square$
    - $\bullet$ Claim 3: $(\forall x\in X, ~(f(x)=\tilde{f}(x)))\land (\forall y\in Y,(g(y)=\tilde{g}(y))) \implies (\forall x\in X, g(f(x))=\tilde{g}(\tilde{f}(x)))$
    - $\Vdash$ $g(f(x))$
    - $=$ { $\forall x\in X, f(x)=\tilde{f}(x)$,\\
                 $~~~$ [[../../Appendix/AxiomOfEquality.org][substitution axiom]] for any two objects of the same type }
      - $g(\tilde{f}(x))$
    - $=$ {$\forall y\in Y, g(y)=\tilde{g}(y)$ and let $y=\tilde{f}(x)$ }
      - $\tilde{g}(\tilde{f}(x))$
    - $\square$
