#+title: Exercise 2.2.2 (Lemma 2.2.10)

Prove [[../lemma-2.2.10.org][Lemma 2.2.10]].
(Hint: use induction. the induction here is somewhat degenerate, in that the induction hypothesis is not actually used, but this does not prevent the argument from remaining valid; cf. the discussion on implication and causality in Appendix A.2.)


- $\bullet$ Show that $\forall a\in\mathbb{N}.~a\neq0\implies \exists!b\in\mathbb{N}.~b\pp=a$.

- $\Vdash$ { Proof by induction on $a$ }

  - $\bullet$ Base case: show that $\forall a\in\mathbb{N}.~a\neq0\implies \exists!b\in\mathbb{N}.~b\pp=a$, when

  - -- $a=0$

  - $\Vdash$ $0\neq0\implies \exists!b\in\mathbb{N}.~b\pp=0$

  - $\equiv$ { implication is vacuously true since the premise $0\neq0$ is false }

    - True

  - $\square$

  - $\bullet$ Inductive step: show that $\forall a\pp\in\mathbb{N}.~a\pp\neq0\implies \exists!b\in\mathbb{N}.~b\pp=a\pp$, when

  - -- $\forall a\in\mathbb{N}.~a\neq0\implies \exists!b\in\mathbb{N}.~b\pp=a$

  - $\Vdash$ $\forall a\pp\in\mathbb{N}.~a\pp\neq0\implies \exists!b\in\mathbb{N}.~b\pp=a\pp$

  - $\equiv$ { Show existence and uniquness of $b$ }

    - $\bullet$ Existence of $b$

    - $\Vdash$ $\forall a\pp\in\mathbb{N}.~a\pp\neq0\implies \exists b\in\mathbb{N}.~b\pp=a\pp$

    - $\equiv$ { Let $b:=a$ }

      - $\forall a\pp\in\mathbb{N}.~a\pp\neq0\implies a\pp=a\pp$

    - $\equiv$ { [[../../Appendix/AxiomOfEquality.org][Reflexive axiom]] }

      - True

    - $\square$

    - $\bullet$ Uniqueness of $b$

    - -- $\forall a\pp\in\mathbb{N}.~a\pp\neq0$
    - $\Vdash$ $(b\pp=a\pp)\land (c\pp=a\pp)$
    - $\Rightarrow$  {$b=a$, $c=a$ by [[../axiom-2.4.org][Axiom 2.4]] }
      - $(b=a)\land (c=a)$
    - $\equiv$   { [[../../Appendix/AxiomOfEquality.org][Symmetry axiom]] : $(c = a) \equiv (a = c)$  }
      - $(b=a)\land (a=c)$
    - $\Rightarrow$   { [[../../Appendix/AxiomOfEquality.org][Transitive axiom]]  }
      - $b=c$
    - $\square$

  - $\cdots$ True
  - $\square$

- $\square$

In the inductive step, the inductive assumption $P(n)$ was not used. Since $P(n\pp)$ is true, $P(n)\implies P(n\pp)$ is always true whether $P(n)$ is true or not
