#+title: Exercise 2.2.1 (Proposition 2.2.5)
#+LATEX_HEADER: \usepackage{amsmath}
#+LATEX_HEADER: \usepackage{amssymb}
#+LATEX_HEADER: \usepackage{a4wide}
#+LATEX_HEADER: \renewcommand{\labelitemi}{}
#+LATEX_HEADER: \renewcommand{\labelitemii}{}
#+LATEX_HEADER: \renewcommand{\labelitemiii}{}
#+LATEX_HEADER: \renewcommand{\labelitemiv}{}
#+LaTeX_HEADER: \newcommand{\pp}{\hspace{-0.5pt}{+}\hspace{-4pt}{+}}
#+LaTeX_HEADER: \usepackage[utf8]{inputenc} \usepackage{titlesec}
#+LaTeX_HEADER: \titleformat{\chapter}[block]{\bfseries\Huge}{}{0em}{}
#+LaTeX_HEADER: \titleformat{\section}[hang]{\bfseries\Large}{}{1em}{\thesection\enspace}
#+OPTIONS: num:nil
#+HTML_HEAD: <style type="text/css">
#+HTML_HEAD:  ol#al { list-style-type: upper-alpha; }
#+HTML_HEAD: </style>

 Prove [[../proposition-2.2.5.org][Proposition 2.2.5]] (Hint: fix two of the variables and induct on the third)

- $\bullet$ Show that $(a+b)+c=a+(b+c)$ for each $a,b,c\in\mathbb{N}$.

- $\Vdash$ { Proof by induction on $a$ }

  - $\bullet$ Base case: show that $(a+b)+c=a+(b+c)$, when

  - $\textnormal{--}$ $a=0$

  - $\Vdash$ $(0+b)+c=0+(b+c)$

  - $\equiv$ { [[../definition-2.2.1.org][Definition 2.2.1]]: $0 + m := m$ }

    - $b+c=b+c$

  - $\square$

  - $\bullet$ Inductive step: show that $((a\pp)+b)+c=(a\pp)+(b+c)$, when

  - $\textnormal{--}$ $(a+b)+c=a+(b+c)$

  - $\Vdash$ $((a\pp)+b)+c$

  - $=$ { [[../definition-2.2.1.org][Definition 2.2.1]]: $(n\pp)+m := (n+m)\pp$ }

    - $((a+b)\pp)+c$

  - $=$ { [[../definition-2.2.1.org][Definition 2.2.1]]: $(n\pp)+m := (n+m)\pp$ }

    - $((a+b)+c)\pp$

  - $=$ { inductive hypothesis,
  - $~~~~$  [[../../Appendix/AxiomOfEquality.org][Substitution Axiom]] $\forall f\forall a\forall b.~ a = b \rightarrow f(a) = f(b)$ }

    - $(a+(b+c))\pp$

  - $=$ { [[../definition-2.2.1.org][Definition 2.2.1]]: $(n\pp)+m := (n+m)\pp$ }

    - $(a\pp)+(b+c)$

  - $\square$

- $\square$
