#+title: Exercise 2.3.5 (Proposition 2.3.9)
#+LATEX_HEADER: \usepackage{amsmath}
#+LATEX_HEADER: \usepackage{amssymb}
#+LATEX_HEADER: \usepackage{a4wide}
#+LATEX_HEADER: \renewcommand{\labelitemi}{}
#+LATEX_HEADER: \renewcommand{\labelitemii}{}
#+LATEX_HEADER: \renewcommand{\labelitemiii}{}
#+LATEX_HEADER: \renewcommand{\labelitemiv}{}
#+LaTeX_HEADER: \newcommand{\pp}{\hspace{-0.5pt}{+}\hspace{-4pt}{+}}
#+LaTeX_HEADER: \usepackage[utf8]{inputenc} \usepackage{titlesec}
#+LaTeX_HEADER: \titleformat{\chapter}[block]{\bfseries\Huge}{}{0em}{}
#+LaTeX_HEADER: \titleformat{\section}[hang]{\bfseries\Large}{}{1em}{\thesection\enspace}
#+OPTIONS: num:nil
#+HTML_HEAD: <style type="text/css">
#+HTML_HEAD:  ol#al { list-style-type: upper-alpha; }
#+HTML_HEAD: </style>

2.3.5 Prove Proposition [[../proposition-2.3.9.org][proposition 2.3.9]] (Hint: fix $q$ and induct on $n$.)

- $\bullet$ Show that $\exists m\exists r\in\mathbb{N}$ such that $0\leq r<q$ and $n=mq+r$, when
- -- $q\neq0$
- $\Vdash$ { Proof by induction on $n$ }
  - $\bullet$ Base case: show that $\exists m\exists r\in\mathbb{N}$ such that $0\leq r<q$ and $n=mq+r$, when
  - -- $n=0$
  - $\Vdash$ $0$
  - $=$ { [[../definition-2.2.1.org][Definition of addition]]: $0+m:=m$;  $0+0=0$ }
    - $0+0$
  - $=$ { [[../definition-2.3.1.org][Definition of multiplication]]: $0\times m:=0$ }
    - $0\times q+0$
  - $\square$
  - $\bullet$ Inductive step: show that $\exists m\exists r\in\mathbb{N}$ such that $0\leq r<q$ and $n\pp=mq+r$, when
  - --$\exists m'\exists r'\in\mathbb{N}$ such that $0\leq r'<q'$ and $n=m'q'+r'$
  - $\Vdash$ $n\pp$
  - $=$ { $n\pp=n+1$ and the inductive hypothesis }
    - $m'q'+r'+1$
  - $=$ { Proof by cases: $r'<q'\implies r'\pp=r'+1\leq q'$ by [[../proposition-2.2.12.org][Proposition 2.2.12]] (e) }
    - $\bullet$ case1: $r'+1=q'$
    - $=$ { substitue $r'+1$ with $q'$ }
      - $m'q'+q'$
    - $=$ { [[../definition-2.3.1.org][Definition of multiplication]]: $(n\pp)\times m:=(n\times m)+m$;  $n\pp=n+1$ }
      - $(m'+1)q'$
    - $=$ { [[../definition-2.2.1.org][Definition of addition]]: $0+m:=m$ }
      - $(m'+1)q'+0$
    - $=$ { Let $m=m'+1,~q=q',~r=0$ }
      - $mq+r$
    - $\square$
    - $\bullet$ case2: $r'+1<q'$
    - $=$ { Let $r=r'+1$ }
      - $m'q'+r$
    - $=$ { Let $m=m',~q=q'$ }
      - $mq+r$
    - $\square$
  - $\square$
- $\square$
