#+title: Exercise 2.3.4
#+LATEX_HEADER: \usepackage{amsmath}
#+LATEX_HEADER: \usepackage{amssymb}
#+LATEX_HEADER: \usepackage{a4wide}
#+LATEX_HEADER: \renewcommand{\labelitemi}{}
#+LATEX_HEADER: \renewcommand{\labelitemii}{}
#+LATEX_HEADER: \renewcommand{\labelitemiii}{}
#+LATEX_HEADER: \renewcommand{\labelitemiv}{}
#+LaTeX_HEADER: \newcommand{\pp}{\hspace{-0.5pt}{+}\hspace{-4pt}{+}}
#+LaTeX_HEADER: \usepackage[utf8]{inputenc} \usepackage{titlesec}
#+LaTeX_HEADER: \titleformat{\chapter}[block]{\bfseries\Huge}{}{0em}{}
#+LaTeX_HEADER: \titleformat{\section}[hang]{\bfseries\Large}{}{1em}{\thesection\enspace}
#+OPTIONS: num:nil
#+HTML_HEAD: <style type="text/css">
#+HTML_HEAD:  ol#al { list-style-type: upper-alpha; }
#+HTML_HEAD: </style>

2.3.4. Prove the identity $(a+b)^2=a^2+2ab+b^2$ for all natural numbers $a,b$.

- $\bullet$ Show that $(a+b)^2=a^2+2ab+b^2$ for all natural numbers $a,b$.
- $\Vdash$ $(a+b)^2$
- $=$ { [[../definition-2.3.11.org][Definition of exponentiation]]: $m^0:=1$; $m^{n\pp}:=m^n\times m$;\\
              $\hspace{1cm} m^2=m^{1\pp}=m^1\times m=m^0\times m\times m=1\times m\times m=m\times m$ }
  - $(a+b)\times (a+b)$
- $=$ { [[../proposition-2.3.4.org][Distributive law]]: $(b+c)a=ba+ca$ }
  - $a(a+b)+b(a+b)$
- $=$ { [[../proposition-2.3.4.org][Distributive law]]: $a(b+c)=ab+ac$ }
  - $aa+ab+ba+bb$
- $=$ { [[../lemma-2.3.2.org][Commutative law]]: $nm=mn$ }
  - $aa+ab+ab+bb$
- $=$ { [[../definition-2.3.1.org][Definition of multiplication]]: $(n\pp)\times m:=n\times m+m$;\\
             $\hspace{1cm} 2m=(1\pp)m=1m+m=m+m$ }
  - $aa+2ab+bb$
- $=$ { [[../definition-2.3.11.org][Definition of exponentiation]]: $m^0:=1$; $m^{n\pp}:=m^n\times m$;\\
  $\hspace{1cm} a^2=a^{1\pp}=a^1a=a^0aa=1aa=aa$  }
  - $a^2+2ab+b^2$
- $\square$
