#+title: Exercise 2.2.3 (Propostion 2.2.12)

#+Author: SoSu
#+LATEX_HEADER: \usepackage{amsmath}
#+LATEX_HEADER: \usepackage{amssymb}
#+LATEX_HEADER: \usepackage{a4wide}
#+LATEX_HEADER: \renewcommand{\labelitemi}{}
#+LATEX_HEADER: \renewcommand{\labelitemii}{}
#+LATEX_HEADER: \renewcommand{\labelitemiii}{}
#+LATEX_HEADER: \renewcommand{\labelitemiv}{}
#+LaTeX_HEADER: \newcommand{\pp}{\hspace{-0.5pt}{+}\hspace{-4pt}{+}}
#+LaTeX_HEADER: \usepackage[utf8]{inputenc} \usepackage{titlesec}
#+LaTeX_HEADER: \titleformat{\chapter}[block]{\bfseries\Huge}{}{0em}{}
#+LaTeX_HEADER: \titleformat{\section}[hang]{\bfseries\Large}{}{1em}{\thesection\enspace}
#+OPTIONS: num:nil


Prove [[../proposition-2.2.12.org][Propostion 2.2.12]]
(Hint: you will need many of the preceding propositions, colloraries, and lemmas.)

(a)

- $\bullet$ Show that $a\geq a$.

- $\Vdash$ $a=a$

- $\equiv$ { [[../lemma-2.2.2.org][Lemma 2.2.2]]: $n+0=n$ }

  - $a=a+0$

- $\equiv$ { [[../definition-2.2.11.org][definition of ordering]]: $n\geq m$ iff $n=m+a$ for some natural number $a$ }

  - $a\geq a$.

- $\square$

(b)

- $\bullet$ Show that $(a\geq b)\land(b\geq c)\implies a\geq c$
- $\Vdash$ $(a\geq b)\land(b\geq c)$
- $\equiv$ { [[../definition-2.2.11.org][definition of ordering]]: $n\geq m$ iff $n=m+a$ for some natural number $a$ }
  - $(a=b+d)\land(b=c+e)$ for some natural numbers $d,e$
- $\equiv$ { Substitute $b$ using $b=c+e$ }
  - $a=c+e+d$ for some natural numbers $d,e$
- $\equiv$ { sum of two natural numbers is a natural number: $e+d=n$ for some natural number $n$ }
  - $a=c+n$ for some natural number $n$
- $\equiv$ { [[../definition-2.2.11.org][definition of ordering]]: $n\geq m$ iff $n=m+a$ for some natural number $a$ }
  - $a\geq c$
- $\square$

(c)

- $\bullet$ Show that $(a\geq b)\land(b\geq a)\implies a=b$
- $\Vdash$ $(a\geq b)\land(b\geq a)$
- $\equiv$ { [[../definition-2.2.11.org][definition of ordering]]: $n\geq m$ iff $n=m+a$ for some natural number $a$ }
  - $(a=b+d)\land(b=a+e)$ for some natural numbers $d,e$

- $\equiv$ { find $d,e$ }
  - $\Vdash$ $(a=b+d)\land(b=a+e)$
  - $\equiv$ { Substitute $b$ using $b=a+e$ }

    - $a=a+e+d$

  - $\equiv$ { [[../lemma-2.2.2.org][Lemma 2.2.2]]: $n+0=n$ }

    - $a+0=a+e+d$

  - $\equiv$ { [[../proposition-2.2.6.org][cancellation law:]] $a+b=a+c\implies b=c$ }

    - $0=e+d$

  - $\equiv$ { [[../corollary-2.2.9.org][Corollary 2.2.9]]: $a+b=0\implies (a=0)\land(b=0)$ }

    - $(d=0)\land(e=0)$

- $\cdots$ $(a=b+0)\land(b=a+0)$

- $\equiv$ { [[../lemma-2.2.2.org][Lemma 2.2.2]]: $n+0=n$ }

  - $(a=b)\land(b=a)$

- $\square$

(d)

- $\bullet$ Show that $a\geq b\iff a+c\geq b+c$
- $\Vdash$ $a\geq b\iff a+c\geq b+c$
  - $\bullet$ Show that $a\geq b\implies a+c\geq b+c$
  - $\Vdash$ $a\geq b$
  - $\equiv$ { [[../definition-2.2.11.org][definition of ordering]]: $n\geq m$ iff $n=m+a$ for some natural number $a$ }
    - $a=b+d$
  - $\equiv$ { [[../../Appendix/AxiomOfEquality.org][Substitution axiom]]: $x=y\implies f(x)=f(y)$ }
    - $a+c=b+d+c$
  - $\equiv$ { [[../proposition-2.2.4.org][addition is commutative]]: $n+m=m+n$ }
    - $a+c=b+c+d$
  - $\equiv$ { [[../definition-2.2.11.org][definition of ordering]]: $n\geq m$ iff $n=m+a$ for some natural number $a$ }
    - $a+c\geq b+c$
  - $\square$
  - $\bullet$ Show that $a+c\geq b+c\implies a\geq b$
  - $\Vdash$ $a+c\geq b+c$
  - $\equiv$ { [[../definition-2.2.11.org][definition of ordering]]: $n\geq m$ iff $n=m+a$ for some natural number $a$ }
    - $a+c=b+c+d$
  - $\equiv$ { [[../proposition-2.2.4.org][addition is commutative]]: $n+m=m+n$ }
    - $a+c=b+d+c$
  - $\equiv$ { [[../proposition-2.2.6.org][cancellation law]]: $a+b=a+c\implies b=c$ }
    - $a=b+d$
  - $\equiv$ { [[../definition-2.2.11.org][definition of ordering]]:$n\geq m$ iff $n=m+a$ for some natural number $a$ }
    - $a\geq d$
  - $\square$
- $\square$
(e)

- $\bullet$ Show that $a<b\iff a\pp\leq b$

- $\Vdash$ $a<b\iff a\pp\leq b$

  - $\bullet$ Show that $a<b\implies a\pp\leq b$

  - $\Vdash$ $a<b$

  - $\equiv$ { [[../definition-2.2.11.org][definition of ordering]]: $m<n$ iff $(m\leq n)\land(m\neq n)$ }

    - $(a\leq b)\land(a\neq b)$

  - $\equiv$ { [[../definition-2.2.11.org][definition of ordering]]: $n\geq m$ iff $n=m+a$ for some natural number $a$ }

    - $(b=a+d)\land(a\neq b)$

  - $\Rightarrow$ { show that when $b=a+d$, $a\neq b\implies d\neq0$ by a proof by contradiction }

    - $\bullet$ Show that there is a contradiction, when
    - -- $a\neq b$

    - -- $d=0$

    - $\Vdash$ $b=a+d$

    - $\equiv$ { assumption: $d=0$ }

      - $b=a+0$

    - $\equiv$ { [[../lemma-2.2.2.org][Lemma 2.2.2]]: $n+0=n$ }

      - $b=a$

    - $\vdash$ { assumption: $a\neq b$ }

      - $\bot$

    - $\square$

  - $\cdots$ $(b=a+d)\land(d\neq0)$

  - $\equiv$ { [[../definition-2.2.7.org][Definition 2.2.7]]: a natural number $n$ is positive iff $n\neq 0$ }

    - $(b=a+d)\land(d\textnormal{ is positive})$

  - $\equiv$ { [[../lemma-2.2.10.org][Lemma 2.2.10]]: For a positive number $n$, $\exists! m,~ m\pp=n$ }

    - $b=a+(m\pp)$

  - $\equiv$ { [[../lemma-2.2.3.org][Lemma 2.2.3]]: $n+(m\pp)=(n+m)\pp$ }

    - $b=(a+m)\pp$

  - $\equiv$ { [[../proposition-2.2.4.org][addition is commutative]]: $n+m=m+n$ }

    - $b=(m+a)\pp$

  - $\equiv$ { [[../lemma-2.2.3.org][Lemma 2.2.3]]: $n+(m\pp)=(n+m)\pp$ }

    - $b=m+(a\pp)$

  - $\equiv$ { [[../proposition-2.2.4.org][addition is commutative]]: $n+m=m+n$  }

    - $b=(a\pp)+m$

  - $\equiv$ { [[../definition-2.2.11.org][definition of ordering]] : $m\leq n$ iff $n=m+a$ }

    - $a\pp\leq b$

  - $\square$

  - $\bullet$ Show that $a\pp\leq b\implies a<b$

  - $\Vdash$ $a\pp\leq b$

  - $\equiv$ { [[../definition-2.2.11.org][definition of ordering]] : $m\leq n$ iff $n=m+a$ }

    - $b=(a\pp)+n$

  - $\equiv$ { [[../definition-2.2.1.org][definition of addition]]: $(n\pp)+m := (n+m)\pp$ }

    - $b=(a+n)\pp$

  - $\equiv$ { [[../lemma-2.2.3.org][Lemma 2.2.3]]: $n+(m\pp)=(n+m)\pp$ }

    - $b=a+(n\pp)$

  - $\Rightarrow$ { show that $b=a+(n\pp)\implies b\neq a$ by a proof by contradiction }

    - $\bullet$ Show that there is a contradiction, when

    - -- $b=a+(n\pp)$
    - -- $b=a$

    - $\Vdash$ $b=a+(n\pp)$

    - $\equiv$ { assumption: $b=a$ }

      - $a=a+(n\pp)$

    - $\equiv$ { [[../lemma-2.2.2.org][Lemma 2.2.2]]: $n+0=n$ }

      - $a+0=a+(n\pp)$

    - $\equiv$ { [[../proposition-2.2.6.org][cancellation law]]: $a+b=a+c\implies b=c$ }

      - $0=n\pp$

    - $\vdash$ { [[../axiom-2.3.org][Axiom 2.3]]: $n\pp\neq0$ for every natural number $n$ }

      - $\bot$

    - $\square$

  - $\cdots$ $(b=a+(n\pp))\land(b\neq a)$
  - $\equiv$ { [[../definition-2.2.11.org][definition of ordering]]: $m<n$ iff $(m\leq n)\land(m\neq n)$ }

    - $a<b$

  - $\square$

- $\square$

(f)
- $\bullet$ Show that $a<b$ iff $b=a+d$ for some positive number $d$
- $\Vdash$ $a<b\iff(b=a+d)\land(d\textnormal{ is positive})$
  - $\bullet$ Show that $a<b\implies (b=a+d)\land(d\textnormal{ is positive})$
  - $\Vdash$ $a<b$
  - $\equiv$ { [[../definition-2.2.11.org][definition of ordering]]: $m\leq n$ iff $n=m+a$,
  - $\hspace{5.3cm}$ $m<n$ iff $(m\leq n)\land(n\neq m)$ }
    - $(b=a+d)\land(a\neq b)$
  - $\Rightarrow$ { show that when $b=a+d$, $a\neq b\implies d\neq0$ by a proof by contradiction }
    - $\bullet$ Show that there is a contradiction, when
    - -- $a\neq b$
    - -- $d=0$
    - $\Vdash$ $b=a+d$
    - $\equiv$ { assumption: $d=0$ }
      - $b=a+0$
    - $\equiv$ { [[../lemma-2.2.2.org][Lemma 2.2.2]]: $n+0=n$ }
      - $b=a$
    - $\vdash$ { assumption: $a\neq b$ }
      - $\bot$
    - $\square$
  - $\cdots$ $(b=a+d)\land(d\neq0)$
  - $\equiv$ { [[../definition-2.2.7.org][Definition 2.2.7]]: a natural number $n$ is positive iff $n\neq 0$ }
    - $(b=a+d)\land(d\textnormal{ is positive})$
  - $\square$
  - $\bullet$ Show that $(b=a+d)\land(d\textnormal{ is positive})\implies a<b$
  - $\Vdash$ $(b=a+d)\land(d\textnormal{ is positive})$
  - $\equiv$ { [[../definition-2.2.7.org][Definition 2.2.7]]: a natural number $n$ is positive iff $n\neq 0$ }
    - $(b=a+d)\land(d\neq0)$
  - $\Rightarrow$ { show that when $b=a+d$, $d\neq0\implies b\neq a$ by a proof by contradiction }
    - $\bullet$ Show that there is a contradiction, when
    - -- $d\neq0$
    - -- $b=a$
    - $\Vdash$ $b=a+d$
    - $\equiv$ { assumption: $b=a$ }
      - $a=a+d$
    - $\equiv$ { [[../lemma-2.2.2.org][Lemma 2.2.2]]: $n+0=n$ }
      - $a+0=a+d$
    - $\equiv$ { [[../proposition-2.2.6.org][cancellation law]]: $a+b=a+c\implies b=c$ }
      - $0=d$
    - $\vdash$ { $d\neq0$ }
      - $\bot$
    - $\square$
  - $\cdots$ $(b=a+d)\land(b\neq a)$
  - $\equiv$ { [[../definition-2.2.11.org][definition of ordering]]: $m\leq n$ iff $n=m+a$,
  - $\hspace{5.3cm}$ $m<n$ iff $(m\leq n)\land(n\neq m)$ }
    - $a<b$
  - $\square$
- $\square$
