#+title: Exercise 2.3.3 (Proporsition 2.3.5 )
#+LATEX_HEADER: \usepackage{amsmath}
#+LATEX_HEADER: \usepackage{amssymb}
#+LATEX_HEADER: \usepackage{a4wide}
#+LATEX_HEADER: \renewcommand{\labelitemi}{}
#+LATEX_HEADER: \renewcommand{\labelitemii}{}
#+LATEX_HEADER: \renewcommand{\labelitemiii}{}
#+LATEX_HEADER: \renewcommand{\labelitemiv}{}
#+LaTeX_HEADER: \newcommand{\pp}{\hspace{-0.5pt}{+}\hspace{-4pt}{+}}
#+LaTeX_HEADER: \usepackage[utf8]{inputenc} \usepackage{titlesec}
#+LaTeX_HEADER: \titleformat{\chapter}[block]{\bfseries\Huge}{}{0em}{}
#+LaTeX_HEADER: \titleformat{\section}[hang]{\bfseries\Large}{}{1em}{\thesection\enspace}
#+OPTIONS: num:nil
#+HTML_HEAD: <style type="text/css">
#+HTML_HEAD:  ol#al { list-style-type: upper-alpha; }
#+HTML_HEAD: </style>

2.3.3. Prove [[../proposition-2.3.5.org][Proposition 2.3.5]] (Hint: modify the proof of [[../proposition-2.2.5.org][Proposition of 2.2.5]] and use the distribution law.)

- $\bullet$ Show that $(a\times b)\times c=a\times(b\times c)$ for each $a,b,c\in\mathbb{N}$.

- $\Vdash$ { Proof by induction on $a$ }

  - $\bullet$ Base case: Show that $(a\times b)\times c=a\times(b\times c)$, when
  - -- $a=0$
  - $\Vdash$ $(0\times b)\times c=0\times(b\times c)$
  - $\equiv$ { [[../definition-2.3.1.org][Definition 2.3.1]]: $\forall m.~0\times m:=0$ }
    - $0\times c=0$
  - $\equiv$ { [[../definition-2.3.1.org][Definition 2.3.1]]: $\forall m.~0\times m:=0$ }
    - $0=0$
  - $\square$

  - $\bullet$ Inductive step: Show that $((a\pp)\times b)\times c=(a\pp)\times(b\times c)$ for each $a,b,c\in\mathbb{N}$., when

  - -- $(a\times b)\times c=a\times(b\times c)$

  - $\Vdash$ $((a\pp)\times b)\times c$

  - $=$ { [[../definition-2.3.1.org][Definition 2.3.1]]: $(n\pp)\times m:=(n\times m)+m$ }
    - $((a\times b)\times b)\times c$
  - $=$ { [[../proposition-2.3.4.org][Proposition 2.3.4]]: $(b+c)a=ba+ca$ }

    - $(a\times b)\times c+b\times c$
  - $=$ { inductive hypothesis }
    - $a\times(b\times c)+(b\times c)$

  - $=$ { [[../definition-2.3.1.org][Definition 2.3.1]]: $(n\pp)\times m:=(n\times m)+m$ }

    - $(a\pp)\times(b\times c)$

  - $\square$

- $\square$
