#+title: Lemma 3.3.12
#+LATEX_HEADER: \usepackage{amsmath}
#+LATEX_HEADER: \usepackage{amssymb}
#+LATEX_HEADER: \usepackage{a4wide}
#+LATEX_HEADER: \renewcommand{\labelitemi}{}
#+LATEX_HEADER: \renewcommand{\labelitemii}{}
#+LATEX_HEADER: \renewcommand{\labelitemiii}{}
#+LATEX_HEADER: \renewcommand{\labelitemiv}{}
#+LaTeX_HEADER: \newcommand{\pp}{\hspace{-0.5pt}{+}\hspace{-4pt}{+}}
#+LaTeX_HEADER: \usepackage[utf8]{inputenc} \usepackage{titlesec}
#+LaTeX_HEADER: \titleformat{\chapter}[block]{\bfseries\Huge}{}{0em}{}
#+LaTeX_HEADER: \titleformat{\section}[hang]{\bfseries\Large}{}{1em}{\thesection\enspace}
#+OPTIONS: num:nil
#+HTML_HEAD: <style type="text/css">
#+HTML_HEAD:  ol#al { list-style-type: upper-alpha; }
#+HTML_HEAD: </style>

*Lemma 3.3.12* (Composition is associative). /Let $f:Z\to W,~g:Y\to Z$, and $h:X\to Y$ be functions.
Then $f\circ(g\circ h)=(f\circ g)\circ h$./

$Proof~by~Tao$. Since $f\circ g$ is a function from $X$ to $Z$, $f\circ(g\circ h)$ is a function from $X$ to $W$.
Simliarly $f\circ g$ is a function from $Y$ to $W$, and hence $(f\circ g)\circ h$ is a function from $X$ to $W$.
Thus $f\circ(g\circ h)$ and $(f\circ g)\circ h$ have the same domain and range. In order to check that they are equal,
we see from [[./definition-3.3.7.org][Definition 3.3.7]] that we have to verify that $(f\circ(g\circ h))(x)=((f\circ g)\circ h)(x)$ for all $x\in X$.
But by [[./definition-3.3.10.org][Definition 3.3.10]]
$$
(f\circ (g\circ h))(x)=f((g\circ h)(x))
$$

$$
=f(g(h(x)))
$$

$$
=(f\circ g)(h(x))
$$

$$
=((f\circ g)\circ h)(x)
$$

as desired. $\square$

$Proof~in~Structured~Derivation~Form$.

- $+$ Notation: $\text{Domain}(f:X\to Y)= X$
- $+$ Notation: $\text{Range}(f:X\to Y)=Y$

- $\bullet$ Show that $f\circ(g\circ h)=(f\circ g)\circ h$, when

- -- $f:Z\to W$
- -- $g:Y\to Z$
- -- $h:X\to Y$

- $\Vdash$ $f\circ(g\circ h)=(f\circ g)\circ h$

- $\equiv$ { Claim 1, Claim2, Claim 3, and [[./definition-3.3.7.org][Definition 3.3.7]],  modus ponens}

  - $\text{True}$

- $\square$

  - $\bullet$ Claim 1. Show that $\text{Domain}(f\circ (g\circ h))=\text{Domain}((f\circ g)\circ h)$

  - $\Vdash$ { show that domains of both sides are $X$ }

    - $\bullet$ Show that $\text{Domain}(f\circ (g\circ h))=X$

    - $\Vdash$ $\text{Domain}(f\circ (g\circ h))$

    - $=$ { let $p=g\circ h$,\\
                       $~~~$ [[./definition-3.3.10.org][Definition 3.3.10]], $p:X\to Z$ }

      - $\text{Domain}(f\circ p)$

    - $=$ { let $q=f\circ p$,\\
                        $~~~$ [[./definition-3.3.10.org][Definition 3.3.10]], $q:X\to W$  }

      - $X$

    - $\square$

    - $\bullet$ Show that $\text{Domain}((f\circ g)\circ h)=X$

    - $\Vdash$ $\text{Domain}((f\circ g)\circ h)$

    - $=$ { let $p=f\circ g$,\\
                        $~~~$ [[./definition-3.3.10.org][Definition 3.3.10]], $p:Y\to W$  }

      - $\text{Domain}(p\circ h)$
    - $=$ { let $q=p\circ h$,\\
                        $~~~$ [[./definition-3.3.10.org][Definition 3.3.10]], $q:Z\to W$  }

      - $X$

    - $\square$

  - $\square$


  - $\bullet$ Claim 2. Show that $\text{Range}(f\circ (g\circ h))=\text{Range}((f\circ g)\circ h)$

  - $\Vdash$ { show that ranges of both sides are $W$ }

    - $\bullet$ Show that $\text{Range}(f\circ (g\circ h))=W$

    - $\Vdash$ $\text{Range}(f\circ (g\circ h))$

    - $=$ { let $p=g\circ h$,\\
                       $~~~$ [[./definition-3.3.10.org][Definition 3.3.10]], $p:X\to Z$ }

      - $\text{Range}(f\circ p)$

    - $=$ { let $q=f\circ p$,\\
                        $~~~$ [[./definition-3.3.10.org][Definition 3.3.10]], $q:X\to W$  }

      - $W$

    - $\square$

    - $\bullet$ Show that $\text{Range}((f\circ g)\circ h)=W$

    - $\Vdash$ $\text{Range}((f\circ g)\circ h)$

    - $=$ { let $p=f\circ g$,\\
                        $~~~$ [[./definition-3.3.10.org][Definition 3.3.10]], $p:Y\to W$  }

      - $\text{Range}(p\circ h)$
    - $=$ { let $q=p\circ h$,\\
                        $~~~$ [[./definition-3.3.10.org][Definition 3.3.10]], $q:Z\to W$  }

      - $W$

    - $\square$

  - $\square$





  - $\bullet$ Claim 3. Show that $\forall x,~(f\circ (g\circ h))(x)=((f\circ g)\circ h)(x)$

  - $\Vdash$ $(f\circ (g\circ h))(x)$

  - $=$ { [[./definition-3.3.10.org][Definition 3.3.10]] }

    - $f((g\circ h)(x))$

  - $=$ { [[./definition-3.3.10.org][Definition 3.3.10]] }

    - $f((g(h(x)))$

  - $=$ { [[./definition-3.3.10.org][Definition 3.3.10]] }

    - $(f\circ g)(h(x))$
  - $=$ { [[./definition-3.3.10.org][Definition 3.3.10]] }

    - $(f\circ g)\circ h)(x)$
  - $\square$
