#+title: Exercise 4.1.4

#+LATEX_HEADER: \usepackage{amsmath}
#+LATEX_HEADER: \usepackage{amssymb}
#+LATEX_HEADER: \usepackage{a4wide}
#+LATEX_HEADER: \renewcommand{\labelitemi}{}
#+LATEX_HEADER: \renewcommand{\labelitemii}{}
#+LATEX_HEADER: \renewcommand{\labelitemiii}{}
#+LATEX_HEADER: \renewcommand{\labelitemiv}{}
#+LaTeX_HEADER: \newcommand{\pp}{\hspace{-0.5pt}{+}\hspace{-4pt}{+}}
#+LaTeX_HEADER: \usepackage[utf8]{inputenc} \usepackage{titlesec}
#+LaTeX_HEADER: \titleformat{\chapter}[block]{\bfseries\Huge}{}{0em}{}
#+LaTeX_HEADER: \titleformat{\section}[hang]{\bfseries\Large}{}{1em}{\thesection\enspace}
#+OPTIONS: num:nil
#+HTML_HEAD: <style type="text/css">
#+HTML_HEAD:  ol#al { list-style-type: upper-alpha; }
#+HTML_HEAD: </style>
*Exercise 4.1.4* /Prove the remaining identities in Proposition 4.1.6. (Hint: one can save some work by using some identities to prove others. For instance, once you know that $xy = yx$, you get for free that $x1 = 1x$, and once you also prove $x(y + z) = xy + xz$, you automatically get $(y + z)x = yx + zx$ for free.)/

- $\bullet$ Show that $x + y = y + x$.

- $\Vdash$ $x + y$

- $=$ { $x = a — b$, $y = c — d$ }

  - $(a — b) + (c — d)$

- $=$ { [[../definition-4.1.2.org][Definition 4.1.2]] }

  - $(a + c) — (b + d)$

- $=$ { Commutativity of the addition on $\mathbb N$ }

  - $(c + a) — (d + b)$

- $=$ { [[../definition-4.1.2.org][Definition 4.1.2]] }

  - $(c — d) + (a — b)$

- $=$ { $x = a — b$, $y = c — d$ }

  - $y + x$

- $\square$

- $\bullet$ Show that $(x + y) + z = x + (y + z)$.

- $\Vdash$ $(x + y) + z$

- $=$ { $x = a — b$, $y = c — d$, $z = e — f$ }

  - $((a — b) + (c — d)) + (e — f)$

- $=$ { [[../definition-4.1.2.org][Definition 4.1.2]] }

  - $((a + c) — (b + d)) + (e — f)$

- $=$ { [[../definition-4.1.2.org][Definition 4.1.2]] }

  - $((a + c) + e) — ((b + d) + f)$

- $=$ { Associativity of the addition on $\mathbb N$ }

  - $(a + (c + e)) — (b + (d + f))$

- $=$ { [[../definition-4.1.2.org][Definition 4.1.2]] }

  - $(a — b) + ((c + e) — (d + f))$

- $=$ { [[../definition-4.1.2.org][Definition 4.1.2]] }

  - $(a — b) + ((c — d) + (e — f))$

- $=$ { $x = a — b$, $y = c — d$, $z = e — f$ }

  - $x + (y + z)$

- $\square$


- $\bullet$ Show that $x + 0 = 0 + x = x$.

- $-$ Let $c\in \mathbb N$ and $0 := c — c$

- $\Vdash$ $x + 0$

- $=$ { $x = a — b$, $0 = c — c$ }

  - $(a — b) + (c — c)$

- $=$ { [[../definition-4.1.2.org][Definition 4.1.2]] }

  - $(a + c) — (b + c)$

- $=$ { [[../definition-4.1.1.org][Definition 4.1.1]], Commutativity and associativity of the addition on $\mathbb N$, $(a + c) + b = a + (b + c)$  }

  - $a — b$

- $=$ { $x = a — b$ }

  - $x$

- $=$ { $x = a — b$ }

  - $a — b$

- $=$ { [[../definition-4.1.1.org][Definition 4.1.1]], Commutativity and associativity of the addition on $\mathbb N$, $a + (c + b) = (c + a) + b$  }

  - $(c + a) — (c + b)$

- $=$ { [[../definition-4.1.2.org][Definition 4.1.2]] }

  - $(c — c) + (a — b)$

- $=$ { $x = a — b$, $0 = c — c$ }

  - $0 + x$

- $\square$

- $\bullet$ (Commutative law of $\mathbb Z$) Show that $xy = yx$.

- $\Vdash$ $xy$

- $=$ { $x = a — b$, $y = c — d$ }

  - $(a — b)(c — d)$

- $=$ { [[../definition-4.1.2.org][Definition 4.1.2]] }

  - $(ac + bd) — (ad + bc)$

- $=$ { Commutativity of the addition and the multiplication on $\mathbb N$ }

  - $(ca + db) — (cb + da)$

- $=$ { [[../definition-4.1.2.org][Definition 4.1.2]] }

  - $(c — d)(a — b)$

- $=$ { $x = a — b$, $y = c — d$ }

  - $yx$

- $\square$

- $\bullet$ Show that $x1_Z = 1_Zx = x$.

- $-$ Let $1_Z = 1_N — 0_N$, $x = a — b$

- $\Vdash$ $x1_Z$

- $=$ { $1_Z = 1_N — 0_N$, $x = a — b$ }

  - $(a — b)(1_N — 0_N)$

- $=$ { [[../definition-4.1.2.org][Definition 4.1.2]] }

  - $(a1_N + b0_N) — (a0_N + b1_N)$

- $=$ { Multiplication on $\mathbb N$ }

  - $a — b$

- $=$ { $x = a — b$ }

  - $x$

- $=$ { $x = a — b$ }

  - $a — b$

- $=$ { Multiplication on $\mathbb N$ }

  - $(1_Na + 0_Nb) — (1_Nb + 0_Na)$

- $=$ { [[../definition-4.1.2.org][Definition 4.1.2]] }

  - $(1_N — 0_N)(a — b)$

- $=$ { $1_Z = 1_N — 0_N$, $x = a — b$ }

  - $1_Zx$

- $\square$

- $\bullet$ (Left distributive law of $\mathbb Z$) Show that $x(y + z) = xy + xz$.

- $-$ Let $x = a — b$, $y = c — d$, $z = e — f$

- $\Vdash$ $x(y + z)$

- $=$ { $x = a — b$, $y = c — d$, $z = e — f$ }

  - $(a — b)((c — d) + (e — f))$

- $=$ { [[../definition-4.1.2.org][Definition 4.1.2]] }

  - $(a — b)((c + e) — (d + f))$

- $=$ { [[../definition-4.1.2.org][Definition 4.1.2]] }

  - $(a(c + e) + b(d + f)) — (a(d + f) + b(c + e))$

- $=$ { Commutative and Distributive law of $\mathbb N$ }

  - $((ac + bd) + (ae + bf)) — ((ad + bc) + (af + be))$

- $=$ { [[../definition-4.1.2.org][Definition 4.1.2]] }

  - $((ac + bd) — (ad + bc)) + ((ae + bf) — (af + be))$

- $=$ { [[../definition-4.1.2.org][Definition 4.1.2]] }

  - $(a — b)(c — d) + (a — b)(e — f)$

- $=$ { $x = a — b$, $y = c — d$, $z = e — f$ }

  - $xy + xz$

- $\square$

- $\bullet$ $(y + z)x = yx + zx$.

- $\Vdash$ $(y + z)x$

- $=$ { Commutative law of $\mathbb Z$ }

  - $x(y + z)$

- $=$ { Left distributive law of $\mathbb Z$ }

  - $xy + xz$

- $=$ { Commutative law of $\mathbb Z$ }

  - $yx + zx$

- $\square$
