#+title: Exercise 4.1.3

#+LATEX_HEADER: \usepackage{amsmath}
#+LATEX_HEADER: \usepackage{amssymb}
#+LATEX_HEADER: \usepackage{a4wide}
#+LATEX_HEADER: \renewcommand{\labelitemi}{}
#+LATEX_HEADER: \renewcommand{\labelitemii}{}
#+LATEX_HEADER: \renewcommand{\labelitemiii}{}
#+LATEX_HEADER: \renewcommand{\labelitemiv}{}
#+LaTeX_HEADER: \newcommand{\pp}{\hspace{-0.5pt}{+}\hspace{-4pt}{+}}
#+LaTeX_HEADER: \usepackage[utf8]{inputenc} \usepackage{titlesec}
#+LaTeX_HEADER: \titleformat{\chapter}[block]{\bfseries\Huge}{}{0em}{}
#+LaTeX_HEADER: \titleformat{\section}[hang]{\bfseries\Large}{}{1em}{\thesection\enspace}
#+OPTIONS: num:nil
#+HTML_HEAD: <style type="text/css">
#+HTML_HEAD:  ol#al { list-style-type: upper-alpha; }
#+HTML_HEAD: </style>

*Exercise 4.1.3* /Show that $(−1) × a = −a$ for every integer $a$./

- $\bullet$ Show that $(−1) × a = −a$ for every integer $a$.

- $\Vdash$ $(−1) × a$

- $=$ { By [[../definition-4.1.1.org][Definition 4.1.1]], $a = b — c$ for some natural number $b$ and $c$; [[../definition-4.1.4.org][Definition 4.1.4]] }

  - $(0 — 1) × (b — c)$

- $=$ { [[../definition-4.1.2.org][Definition 4.1.2]] }

  - $(0b + 1c)—(0c + 1b)$

- $=$ { Multiplication on $\mathbb N$ }

  - $(c — b)$

- $=$ { [[../definition-4.1.4.org][Definition 4.1.4]] }

  - $−(b — c)$

- $=$ { $a = b — c$ }

  - $−a$

- $\square$
