#+title: Appendix

* Appendix A
** A.1
$X\implies Y$ (Y is true if X is true) is equivalent to $\lnot X\lor Y$ or $\lnot(X\land\lnot Y)$.

The truth table of logical implication

#+ATTR_LATEX: :align |c|c|c|c|c|
|-----+-----+---------------+-----------+-----------------|
| $X$ | $Y$ | $X\implies Y$ | $\lnot X$ | $\lnot X\lor Y$ |
|-----+-----+---------------+-----------+-----------------|
| T   | T   | T             | F         | T               |
| T   | F   | F             | F         | F               |
| F   | T   | T             | T         | T               |
| F   | F   | T             | T         | T               |
|-----+-----+---------------+-----------+-----------------|

*** A.1.1

- $\bullet$ What is the negation of the statement "either X is true, or Y is true, but not both"?

- $(1)$ Logical expression for "either X is true or Y is true" is $X \lor Y$

- $(2)$ Logical expression for "not both" is $\lnot(X \land Y)$

- $(3)$ Logical expression for "either X is true or Y is true, /but/ not both" is $(X \lor Y) \land\lnot(X\land Y)$

- $\Vdash$ $\lnot((X \lor Y) \land\lnot(X\land Y))$

- $\equiv$ {  Distribution of negation over $\land$:
                          ${}^\forall p {}^\forall q. \ \lnot (p \land q) \equiv (\lnot p \lor \lnot q)$
                       }

      $\lnot(X \lor Y) \lor \lnot(\lnot(X\land Y))$

- $\equiv$ {  Double Negation:
                          ${}^\forall p. \ \lnot \lnot p \equiv p$
                      }

      $\lnot(X \lor Y) \lor (X\land Y)$

- $\equiv$ {  Distribution of negation over $\lor$:
                          ${}^\forall p {}^\forall q. \ \lnot (p \lor q) \equiv (\lnot p \land \lnot q)$
                       }

     $(\lnot X \land \lnot Y) \lor (X\land Y)$

- $\equiv$ {  By converting the logical expression into a sentence }

      Neither X is true nor Y is true or both are true

- $\square$


#+ATTR_LATEX: :align |c|c|c|c|c|c|c|c|
|-----+-----+------------+------------+-------------------+-----------------------------------+-------------------+----------------------------------------|
| $X$ | $Y$ | $X \lor Y$ | $X\land Y$ | $\lnot(X\land Y)$ | $(X \lor Y) \land\lnot(X\land Y)$ | $\lnot(X \lor Y)$ | $(\lnot X\land\lnot Y)\lor (X\land Y)$ |
|-----+-----+------------+------------+-------------------+-----------------------------------+-------------------+----------------------------------------|
| T   | T   | T          | T          | F                 | F                                 | F                 | T                                      |
| T   | F   | T          | F          | T                 | T                                 | F                 | F                                      |
| F   | T   | T          | F          | T                 | T                                 | F                 | F                                      |
| F   | F   | F          | F          | T                 | F                                 | T                 | T                                      |
|-----+-----+------------+------------+-------------------+-----------------------------------+-------------------+----------------------------------------|


*** A.1.2
What is the negation of the statement "X is true if and only if Y is true"? (There may be multiple ways to phrase this negation).

$$
X\implies Y=\lnot(X\land\lnot Y)
$$

$$
X \iff Y = (X\implies Y)\land(Y\implies X)=\lnot(X\land\lnot Y)\land\lnot(Y\land\lnot X)
$$

$$
\lnot(\lnot(X\land\lnot Y)\land\lnot(Y\land\lnot X))=(X\land\lnot Y)\lor(Y\land\lnot X)
$$

Either X is true and Y is false, or X is false and Y is true.


|$X$|$Y$|$\lnot X$|$\lnot Y$|$\lnot X\lor Y$|$\lnot Y\lor X$|$(\lnot X\lor Y)\land(\lnot Y\lor X)$|$X\land\lnot Y$|$Y\land\lnot X$|$(X\land\lnot Y)\lor(Y\land\lnot X)$|
| T | T | F       | F       | T             | T             |T                                    |F              |F              |F|
| T | F | F       | T       | F             | T             |F                                    |T              | F             |T|
| F | T | T       | F       | T             | F             |F                                    |F              | T             |T|
| F | F | T       | T       | T             | T             |T                                    |F              | F             |F|

*** A.1.3
Suppose that you have shown that whenever X is true, the Y is true, and whenever Y is false, then X is false. Have you now demonstrated that X is true if and only if Y is true? Explain.

$$
X\iff Y = (X\implies Y)\land(Y\implies X)
$$

$\lnot X\implies\lnot Y$ is contraposition of $Y\implies X$. Hence,

$$
(X\implies Y)\land((\lnot X\implies\lnot Y)=(X\implies Y)\land(Y\implies X)=X\iff Y
$$

It demonstrates that X is true if and only if Y is true.

|$X$|$Y$|$X\implies Y$|$Y\implies X$|$\lnot X$|$\lnot Y$|$\lnot X\implies\lnot Y$|$(X\implies Y)\land(Y\implies X)$|$(X\implies Y)\land(\lnot X\implies\lnot Y)$|
|T  |T  |T            |T            |F        |F        |T                       |T                                |T                                           |
|T  |F  |F            |T            |F        |T        |T                       |F                                |F                                           |
|F  |T  |T            |F            |T        |F        |F                       |F                                |F                                           |
|F  |F  |T            |T            |T        |T        |T                       |T                                |T                                           |

*** A.1.4
Suppose that you have shown that whenever X is true, then Y is true, and whenever Y is false, then X is false. Have you now demonstrated that X is true if and only if Y is true? Explain.

$$
X\iff Y = (X\implies Y)\land(Y\implies X)
$$

$\lnot Y\implies\lnot X$ is contraposition of $X\implies Y$. Hence,

$$
(X\implies Y)\land((\lnot Y\implies\lnot X)=(X\implies Y)\land(X\implies Y)=X\implies Y
$$

It does not demonstrate that X is true if and only if Y is true.

|$X$|$Y$|$X\implies Y$|$Y\implies X$|$\lnot X$|$\lnot Y$|$\lnot Y\implies\lnot X$|$(X\implies Y)\land(Y\implies X)$|$(X\implies Y)\land(\lnot Y\implies\lnot X)$|
|T  |T  |T            |T            |F        |F        |T                       |T                                |T                                           |
|T  |F  |F            |T            |F        |T        |F                       |F                                |F                                           |
|F  |T  |T            |F            |T        |F        |T                       |F                                |T                                           |
|F  |F  |T            |T            |T        |T        |T                       |T                                |T                                           |

*** A.1.5
Suppose you know that X is true if and only if Y true, and you know that Y is true if and only if Z is true. Is this enough to show that X, Y, Z are all logically quivalent? Explain.


|$A$|$B$|$A\iff B$|
|T  |T  |T        |
|T  |F  |F        |
|F  |T  |F        |
|F  |F  |T        |


X iff Y states that X and Y are logically equivalent, and Y iff Z states that Y and Z are logically equivalent. Therefore, X iff Y and Y iff Z state that X, Y, Z are logically equivalent.

*** A.1.6
Soppose you know that whenever X is true, then Y is true; that whenever Y is true, then Z is true; and whenever Z is true, then X is true. Is this enough to show that X, Y, Z are all logically equivalent? Explain.

$$
(X\implies Y)\land(Y\implies Z)\land(Z\implies X)
$$

|$X$|$Y$|$Z$|$X\implies Y$|$Y\implies Z$|$Z\implies X$|$(X\implies Y)\land(Y\implies Z)\land(Z\implies X)$|
|T  |T  |T  |T            |T            |T            |T                                                  |
|T  |T  |F  |T            |F            |T            |F                                                  |
|T  |F  |T  |F            |T            |T            |F |
|T  |F  |F  |F            |T            |T            |F |
|F  |T  |T  |T            |T            |F            |F |
|F  |T  |F  |T            |F            |T            |F |
|F  |F  |T  |T            |T            |F            |F |
|F  |F  |F  |T            |T            |T            |T |

$(X\implies Y)\land(Y\implies Z)\land(Z\implies X)$ states that X, Y, Z are logically equivalent.
