#+Title: Tao solution: Chapter 2
#+Author: SoSu
#+LATEX_HEADER: \usepackage{amsmath}
#+LATEX_HEADER: \usepackage{amssymb}
#+LATEX_HEADER: \usepackage{a4wide}
#+LATEX_HEADER: \renewcommand{\labelitemi}{}
#+LATEX_HEADER: \renewcommand{\labelitemii}{}
#+LATEX_HEADER: \renewcommand{\labelitemiii}{}
#+LATEX_HEADER: \renewcommand{\labelitemiv}{}
#+LaTeX_HEADER: \newcommand{\pp}{\hspace{-0.5pt}{+}\hspace{-4pt}{+}}
#+LaTeX_HEADER: \usepackage[utf8]{inputenc} \usepackage{titlesec}
#+LaTeX_HEADER: \titleformat{\chapter}[block]{\bfseries\Huge}{}{0em}{}
#+LaTeX_HEADER: \titleformat{\section}[hang]{\bfseries\Large}{}{1em}{\thesection\enspace}
#+OPTIONS: num:nil


* Exercises 2.2
** 2.2.1. Prove Proposition 2.2.5 (Hint: fix two of the variables and induct on the third)

*Proposition 2.2.5* /(Addition is associative)/

/For any natural numbers $a,b,c$,
we have $(a+b)+c=a+(b+c)$./

- $\bullet$ Show that $(a+b)+c=a+(b+c)$ for each $a,b,c\in\mathbb{N}$.

- $\Vdash$ { Proof by induction on $a$ }

  - $\bullet$ Base case: show that $(a+b)+c=a+(b+c)$, when

  - $\textnormal{--}$ $a=0$

  - $\Vdash$ $(a+b)+c=a+(b+c)$

  - $\equiv$ { substitute assumption $a=0$ }

    - $(0+b)+c=0+(b+c)$

  - $\equiv$ { Definition 2.2.1: ${}^\forall m.~ 0 + m := m$ }

    - $b+c=b+c$

  - $\square$

  - $\bullet$ Inductive step: show that $((a\pp)+b)+c=(a\pp)+(b+c)$, when

  - $\textnormal{--}$ $(a+b)+c=a+(b+c)$

  - $\Vdash$ $((a\pp)+b)+c$

  - $=$ { Definition 2.2.1: ${}^\forall n{}^\forall m.~ (n\pp)+m := (n+m)\pp$ }

    - $((a+b)\pp)+c$

  - $=$ { Definition 2.2.1: ${}^\forall n{}^\forall m.~ (n\pp)+m := (n+m)\pp$ }

    - $((a+b)+c)\pp$

  - $=$ { inductive hypothesis,
  - $~~~~$  Substitution Axiom ${}^\forall f{}^\forall a{}^\forall b.~ a = b \rightarrow f(a) = f(b)$}

    - $(a+(b+c))\pp$

  - $=$ { Definition 2.2.1: ${}^\forall n{}^\forall m.~ (n\pp)+m := (n+m)\pp$ }

    - $(a\pp)+(b+c)$

  - $\square$

- $\square$

** 2.2.2. Prove Lemma 2.2.10.
(Hint: use induction. the induction here is somewhat degenerate, in that the induction hypothesis is not actually used, but this does not prevent the argument from remaining valid; cf. the discussion on implication and causality in Appendix A.2.)

*Lemma 2.2.10.*

/Let $a$ be a positive number. Then there exists exactly one natural number $b$ such that $b\pp=a$./


- $\bullet$ Show that $\forall a\in\mathbb{N}:a\neq0\implies \exists!b\in\mathbb{N}:b\pp=a$.

- $\Vdash$ { Proof by induction on $a$}

  - $\bullet$ Base case: show that $\forall a\in\mathbb{N}:a\neq0\implies \exists!b\in\mathbb{N}:b\pp=a$, when

  - $\textnormal{--}$ $a=0$

  - $\Vdash$ $0\neq0\implies \exists!b\in\mathbb{N}:b\pp=0$

  - $\equiv$ { implication is vacuously true since $0\neq0$ is false }

    - True

  - $\square$

  - $\bullet$ Inductive step: show that $\forall a\pp\in\mathbb{N}:a\pp\neq0\implies \exists!b\in\mathbb{N}:b\pp=a\pp$, when

  - $\textnormal{--}$ $\forall a\in\mathbb{N}:a\neq0\implies \exists!b\in\mathbb{N}:b\pp=a$

  - $\Vdash$ $\forall a\pp\in\mathbb{N}:a\pp\neq0\implies \exists!b\in\mathbb{N}:b\pp=a\pp$

  - $\equiv$ { Show existence and uniquness of $b$ }

    - $\bullet$ Existence of $b$

    - $\Vdash$ $\forall a\pp\in\mathbb{N}:a\pp\neq0\implies \exists b\in\mathbb{N}:b\pp=a\pp$

    - $\equiv$ { Let $b:=a$ }

      - $\forall a\pp\in\mathbb{N}:a\pp\neq0\implies a\pp=a\pp$

    - $\equiv$ { Reflexive axiom }

      - True

    - $\square$

    - $\bullet$ Uniqueness of $b$

    - $\textnormal{--}$ $\forall a\pp\in\mathbb{N}:a\pp\neq0$
    - $\Vdash$           $\forall b, \forall c\in\mathbb{N}:(b\pp=a\pp)\land (c\pp=a\pp)$
    - $\Rightarrow$  {$b=a$, $c=a$ by Axiom 2.4 }
      - $\forall b, \forall c\in\mathbb{N}:(b=a)\land (c=a)$
    - $\equiv$   { Symmetry axiom : $(c = a) \equiv (a = c)$  }
      - $\forall b, \forall c\in\mathbb{N}:(b=a)\land (a=c)$
    - $\Rightarrow$   { Transitive axiom  }
      - $b=c$
    - $\square$

  - $\cdots$ True
  - $\square$

- $\square$

In the inductive step, the inductive assumption $P(n)$ was not used. Since $P(n\pp)$ is true, $P(n)\implies P(n\pp)$ is always true whether or not $P(n)$ is true

** 2.2.3. Prove Propostion 2.2.12
(Hint: you will need many of the preceding propositions, colloraries, and lemmas.)

*Propostion 2.2.12* (Basic properties of order for natural numbers)
/let $a,b,c$ be natural numbers. Then/

- /(a) (Order is reflexive) $a\geq a$/

- /(b) (Order is transitive) If $a\geq b$ and $b\geq c$, then $a\geq c$/

- /(c) (Order is anti-symmetric) If $a\geq b$ and $b\geq a$, then $a=b$/

- /(d) (Addition preserves order) $a\geq b$ only and only if $a+c\geq b+c$/

- /(e) $a<b$ if and only if $a\pp\leq b$/

- /(f) $a<b$ if and only if $b=a+d$ for some positive number $a$/


(a)

- $\bullet$ Show that $a\geq a$.

- $\Vdash$ $a=a$

- $\equiv$ { Lemma 2.2.2: $n+0=n$ }

  - $a=a+0$

- $\equiv$ {Definition 2.2.11: $n\geq m$ iff $n=m+a$ for some natural number $a$}

  - $a\geq a$.

- $\square$

(b)

- $\bullet$ Show that $(a\geq b)\land(b\geq c)\implies a\geq c$
- $\Vdash$ $(a\geq b)\land(b\geq c)$
- $\equiv$ { Definition 2.2.11: $n\geq m$ iff $n=m+a$ for some natural number $a$ }
  - $(a=b+d)\land(b=c+e)$ for some natural numbers $d,e$
- $\equiv$ { Substitute $b$ using $b=c+e$ }
  - $a=c+e+d$ for some natural numbers $d,e$
- $\equiv$ { sum of two natural numbers is a natural number: $e+d=n$ for some natural number $n$ }
  - $a=c+n$ for some natural number $n$
- $\equiv$ { Definition 2.2.11: $n\geq m$ iff $n=m+a$ for some natural number $a$ }
  - $a\geq c$
- $\square$

(c)

- $\bullet$ Show that $(a\geq b)\land(b\geq a)\implies a=b$
- $\Vdash$ $(a\geq b)\land(b\geq a)$
- $\equiv$ { Definition 2.2.11:$n\geq m$ iff $n=m+a$ for some natural number $a$ }
  - $(a=b+d)\land(b=a+e)$ for some natural numbers $d,e$

- $\equiv$ { find $d,e$ }
  - $\Vdash$ $(a=b+d)\land(b=a+e)$
  - $\equiv$ { Substitute $b$ using $b=a+e$ }

    - $a=a+e+d$

  - $\equiv$ { Lemma 2.2.2: ${}^\forall n,~n+0=n$ }

    - $a+0=a+e+d$

  - $\equiv$ { Proposition 2.2.6: Cancelation law, ${}^\forall a{}^\forall b{}^\forall c\in\mathbb{N},~ a+b=a+c\implies b=c$ }

    - $0=e+d$

  - $\equiv$ { Corollary 2.2.9: ${}^\forall a{}^\forall b\in\mathbb{N},~a+b=0\implies (a=0)\land(b=0)$ }

    - $(d=0)\land(e=0)$

- $\cdots$ $(a=b+0)\land(b=a+0)$

- $\equiv$ { Lemma 2.2.2:${}^\forall n,~n+0=n$ }

  - $(a=b)\land(b=a)$

- $\square$

(d)

- $\bullet$ Show that $a\geq b\iff a+c\geq b+c$
- $\Vdash$ $a\geq b\iff a+c\geq b+c$
  - $\bullet$ Show that $a\geq b\implies a+c\geq b+c$
  - $\Vdash$ $a\geq b$
  - $\equiv$ { Definition 2.2.11:$n\geq m$ iff $n=m+a$ for some natural number $a$ }
    - $a=b+d$
  - $\equiv$ { Substitution axiom: $x=y\implies f(x)=f(y)$ }
    - $a+c=b+d+c$
  - $\equiv$ { Proposition 2.2.4: $n+m=m+n$ }
    - $a+c=b+c+d$
  - $\equiv$ { Definition 2.2.11:$n\geq m$ iff $n=m+a$ for some natural number $a$ }
    - $a+c\geq b+c$
  - $\square$
  - $\bullet$ Show that $a+c\geq b+c\implies a\geq b$
  - $\Vdash$ $a+c\geq b+c$
  - $\equiv$ { Definition 2.2.11:$n\geq m$ iff $n=m+a$ for some natural number $a$ }
    - $a+c=b+c+d$
  - $\equiv$ { Proposition 2.2.4: $n+m=m+n$ }
    - $a+c=b+d+c$
  - $\equiv$ { Proposition 2.2.6: $a+b=a+c\implies b=c$ }
    - $a=b+d$
  - $\equiv$ { Definition 2.2.11:$n\geq m$ iff $n=m+a$ for some natural number $a$ }
    - $a\geq d$
  - $\square$
- $\square$
(e)

- $\bullet$ Show that $a<b\iff a\pp\leq b$

- $\Vdash$ $a<b\iff a\pp\leq b$

  - $\bullet$ Show that $a<b\implies a\pp\leq b$

  - $\Vdash$ $a<b$

  - $\equiv$ { Definition 2.2.11: $m<n$ iff $(m\leq n)\land(m\neq n)$ }

    - $(a\leq b)\land(a\neq b)$

  - $\equiv$ { Definition 2.2.11:$n\geq m$ iff $n=m+a$ for some natural number $a$ }

    - $(b=a+d)\land(a\neq b)$

  - $\equiv$ { show that $d\neq0$ }

    - $\bullet$ For sake of constradiction, suppose that

    - $\textnormal{--}$ $d=0$

    - $\Vdash$ $b=a+d$

    - $\equiv$ { assumption $d=0$ }

      - $b=a+0$

    - $\equiv$ { Lemma 2.2.2: $n+0=n$ }

      - $b=a$

    - $\equiv$ { $a\neq b$ }

      - Contradiction

    - $\square$

  - $\cdots$ $(b=a+d)\land(d\neq0)$

  - $\equiv$ { Definition 2.2.7: a natural number $n$ is positive iff $n\neq 0$ }

    - $(b=a+d)\land(d\textnormal{ is positive})$

  - $\equiv$ { Lemma 2.2.10: For a positive number $n$, $\exists! m,~ m\pp=n$ }

    - $b=a+(m\pp)$

  - $\equiv$ { Lemma 2.2.3: $n+(m\pp)=(n+m)\pp$ }

    - $b=(a+m)\pp$

  - $\equiv$ { Proposition 2.2.4: $n+m=m+n$ }

    - $b=(m+a)\pp$

  - $\equiv$ { Lemma 2.2.3: $n+(m\pp)=(n+m)\pp$ }

    - $b=m+(a\pp)$

  - $\equiv$ { Proposition 2.2.4: $n+m=m+n$  }

    - $b=(a\pp)+m$

  - $\equiv$ { Definition 2.2.11 : $m\leq n$ iff $n=m+a$ }

    - $a\pp\leq b$

  - $\square$

  - $\bullet$ Show that $a\pp\leq b\implies a<b$

  - $\Vdash$ $a\pp\leq b$

  - $\equiv$ { Definition 2.2.11 : $m\leq n$ iff $n=m+a$ }

    - $b=(a\pp)+n$

  - $\equiv$ { Deifinition 2.2.1: $(n\pp)+m := (n+m)\pp$ }

    - $b=(a+n)\pp$

  - $\equiv$ { Lemma 2.2.3: $n+(m\pp)=(n+m)\pp$ }

    - $b=a+(n\pp)$

  - $\equiv$ { show that $b=a+(n\pp)\implies b\neq a$ }

    - $\bullet$ For sake of contradiction, suppose that

    - $\textnormal{--}$ $b=a$

    - $\Vdash$ $b=a+(n\pp)$

    - $\equiv$ { assumption $b=a$ }

      - $a=a+(n\pp)$

    - $\equiv$ { Lemma 2.2.2: $n+0=n$ }

      - $a+0=a+(n\pp)$

    - $\equiv$ { Proposition 2.2.6: $a+b=a+c\implies b=c$ }

      - $0=n\pp$

    - $\equiv$ { Axiom 2.3: $n\pp\neq0$ for every natural number $n$ }

      - Contradiction

    - $\square$

  - $\cdots$ $(b=a+(n\pp))\land(b\neq a)$
  - $\equiv$ { Definition 2.2.11: $m<n$ iff $(m\leq n)\land(m\neq n)$ }

    - $a<b$

  - $\square$

- $\square$

(f)
- $\bullet$ Show that $a<b$ iff $b=a+d$ for some positive number $d$
- $\Vdash$ $a<b\iff(b=a+d)\land(d\textnormal{ is positive})$
  - $\bullet$ Show that $a<b\implies (b=a+d)\land(d\textnormal{ is positive})$
  - $\Vdash$ $a<b$
  - $\equiv$ { Definition 2.2.11: $m\leq n$ iff $n=m+a$,
  - $~~~~~~~~~~~~~~~~~~$ $m<n$ iff $(m\leq n)\land(n\neq m)$ }
    - $(b=a+d)\land(a\neq b)$
  - $\equiv$ { show that $d\neq0$ }
    - $\bullet$ For sake of contradiction, suppose that
    - $\textnormal{--}$ $d=0$
    - $\Vdash$ $b=a+d$
    - $\equiv$ { assumption $d=0$ }
      - $b=a+0$
    - $\equiv$ { Lemma 2.2.2: $n+0=n$ }
      - $b=a$
    - $\equiv$ { $a\neq b$ }
      - Contradiction
    - $\square$
  - $\cdots$ $(b=a+d)\land(d\neq0)$
  - $\equiv$ { Definition 2.2.7: a natural number $n$ is positive iff $n\neq 0$ }
    - $(b=a+d)\land(d\textnormal{ is positive})$
  - $\square$
  - $\bullet$ Show that $(b=a+d)\land(d\textnormal{ is positive})\implies a<b$
  - $\Vdash$ $(b=a+d)\land(d\textnormal{ is positive})$
  - $\equiv$ { Definition 2.2.7: a natural number $n$ is positive iff $n\neq 0$ }
    - $(b=a+d)\land(d\neq0)$
  - $\equiv$ { show that $b\neq a$ }
    - $\bullet$ For sake of contradiction, suppose that
    - $\textnormal{--}$ $b=a$
    - $\Vdash$ $b=a+d$
    - $\equiv$ { assumption $b=a$ }
      - $a=a+d$
    - $\equiv$ { Lemma 2.2.2: $n+0=n$ }
      - $a+0=a+d$
    - $\equiv$ { Proposition 2.2.6: $a+b=a+c\implies b=c$ }
      - $0=d$
    - $\equiv$ { $d\neq0$ }
      - Contradiction
    - $\square$
  - $\cdots$ $(b=a+d)\land(b\neq a)$
  - $\equiv$ { Definition 2.2.11: $m\leq n$ iff $n=m+a$,
  - $~~~~~~~~~~~~~~~~~~$ $m<n$ iff $(m\leq n)\land(n\neq m)$ }
    - $a<b$
  - $\square$
- $\square$

** 2.2.4. Justify the three statments marked (why?) in the proof of Proposition 2.2.13.
*Proposition 2.2.13* (Trichotomy of order for natural numbers). /Let $a$ and $b$ be natural numbers. Then excactly one of the following statements is true: $a<b, a=b$, or $a>b$./


When $a=0$ we have $0\leq b$ for all $b$.
- $\bullet$ Show that $0\leq b$ for all $b$
- $\Vdash$ $b=b$
- $\equiv$ { Definition 2.2.1: $0+m:=m$ }
  - $b=0+b$
- $\equiv$ { Definition 2.2.11: $m\leq n$ iff $n=m+a$ for some natural number $a$ }
  - $b\geq 0$
- $\square$

If $a>b$, then $a\pp>b$.
- $\bullet$ Show that $a>b\implies a\pp>b$
- $\Vdash$ $a>b$
- $\equiv$ { Definition 2.2.11: $m<n$ iff $(m\leq n)\land(m\neq n)$ }
  - $(a\geq b)\land(a\neq b)$
- $\equiv$ { Proposition 2.2.12 (d): $a\geq b$ iff $a+c\geq b+c$ }
  - $(a+1\geq b+1)\land(a\neq b)$
- $\equiv$ { $n\pp=n+1$ }
  - $(a\pp\geq b\pp)\land(a\neq b)$
- $\equiv$ { Propostion 2.2.12 (e): $a<b$ iff $a\pp\leq b$ }

  - $(a\pp>b)\land(a\neq b)$

- $\square$

If $a=b$, then $a\pp>b$.
- $\bullet$ Show that $a=b\implies a\pp>b$
- $\Vdash$ $a=b$
- $\equiv$ { Substitution axiom: $a=b\implies f(a)=f(b)$ }
  - $a\pp=b\pp$
- $\equiv$ { $n\pp=n+1$ }
  - $a\pp=b+1$
- $\equiv$ { Proposition 2.2.12 (f): $a<b$ iff $b=a+d$ for some natural number $d$ }
  - $a\pp>b$
- $\square$
